theories/ARL/Lib/FreshExtras.v
@@ -1,4 +1,5 @@
 From stdpp Require Import prelude fin_maps.
+From ARL.Lib Require Import Lists.
 
 Section refresh_map.
 
@@ -15,27 +16,34 @@ Fixpoint refresh_list'
 Definition refresh_list (to_rename to_avoid : KSet) : list (K * K) :=
   refresh_list' (elements to_rename) (to_avoid ∪ to_rename).
 
-Lemma refresh_list_replacements_are_fresh' (orig : list K) (X : KSet) :
-  forall y, y ∈ (map snd (refresh_list' orig X)) -> y ∉ X.
+Lemma refresh_list_replacements_are_fresh' (orig : list K) (X : KSet) P `{forall xy, Decision (P xy)}:
+  forall y, y ∈ (map snd (filter P (refresh_list' orig X))) -> y ∉ X.
 Proof.
   revert X; induction orig; [by inversion 1 | ].
-  cbn; intros ? ?; rewrite elem_of_cons; intros [-> | Hy].
+  intros ? ?; rewrite elem_of_list_fmap; intros (xy & -> & Hfilter).
+  apply elem_of_list_filter in Hfilter as [Hp Hxy]; cbn in Hxy.
+  apply elem_of_cons in Hxy as [-> | Hy].
   - by apply is_fresh.
-  - apply IHorig in Hy.
-    by contradict Hy; apply elem_of_union; right.
+  - apply not_elem_of_union with (X := {[fresh X]}),
+      IHorig, elem_of_list_fmap.
+    eexists; split; [done |].
+    by apply elem_of_list_filter.
 Qed.
 
 Lemma refresh_list_replacements_nodup' :
-  forall orig X , NoDup (map snd (refresh_list' orig X)).
+  forall orig X P `{forall xy, Decision (P xy)},
+    NoDup (map snd (filter P (refresh_list' orig X))).
 Proof.
-  induction orig; [by constructor |]; cbn.
+  induction orig; [by constructor |]; cbn; intros.
+  case_decide; [| by apply IHorig].
   constructor; [| by apply IHorig].
   intro Hx; apply refresh_list_replacements_are_fresh' in Hx.
   by contradict Hx; rewrite elem_of_union, elem_of_singleton; left.
 Qed.
 
 Lemma refresh_list_replacements_nodup :
-  forall orig X, NoDup (map snd (refresh_list orig X)).
+  forall orig X P `{forall xy, Decision (P xy)},
+    NoDup (map snd (filter P (refresh_list orig X))).
 Proof.
   by intros orig X; apply refresh_list_replacements_nodup'.
 Qed.
@@ -58,13 +66,16 @@ Proof.
   apply NoDup_app; split_and!.
   - by rewrite refresh_list_fst; apply NoDup_elements.
   - intro x; rewrite refresh_list_fst, elem_of_elements; intros Hx1 Hx2.
-    eapply refresh_list_replacements_are_fresh'; [done |].
+    eapply refresh_list_replacements_are_fresh' with (P := const True);
+      [by rewrite list_filter_True |].
     by rewrite elem_of_union; right.
-  - apply refresh_list_replacements_nodup.
+  - rewrite <- (list_filter_True (refresh_list orig X)).
+    by apply refresh_list_replacements_nodup.
 Qed.
 
 Lemma refresh_list_replacements_orig :
-  forall orig X, list_to_set (map snd (refresh_list orig X)) ## orig.
+  forall orig X P `{forall xy, Decision (P xy)},
+    list_to_set (map snd (filter P (refresh_list orig X))) ## orig.
 Proof.
   intros.
   pose proof (Hnodup := refresh_list_nodup orig X).
@@ -72,11 +83,14 @@ Proof.
   intros x Hrepl Horig.
   apply (Hnodup x).
   - by rewrite refresh_list_fst, elem_of_elements.
-  - by apply elem_of_list_to_set in Hrepl.
+  - apply elem_of_list_to_set, elem_of_list_fmap in Hrepl
+      as (xy & -> & Hxy).
+    apply elem_of_list_fmap; eexists; split; [done |].
+    by apply elem_of_list_filter in Hxy as [].
 Qed.
 
-Lemma refresh_list_replacements_avoid (orig X : KSet) :
-  list_to_set (map snd (refresh_list orig X)) ## X.
+Lemma refresh_list_replacements_avoid (orig X : KSet) P `{forall xy, Decision (P xy)} :
+  list_to_set (map snd (filter P (refresh_list orig X))) ## X.
 Proof.
   intro y; rewrite elem_of_list_to_set; intro Hy.
   apply refresh_list_replacements_are_fresh' in Hy.
