theories/ARL/QARS/Matching.v
@@ -12,6 +12,11 @@ Context
   (NameSet : Type)
   `{FinSet Name NameSet}.
 
+(** We say that a set of variables <<dependent_vars>> contains all the variables
+that the associated patterns to a set of <<interesting_vars>> of a
+substitution <<s>> depend on, if each of those patterns only depends on the set
+of <<dependent_vars>>.
+*)
 Definition substitution_dependent_vars
   (s : substitution Name) (interesting_vars dependent_vars : NameSet) : Prop :=
   set_Forall (fun x => pattern_dependent_vars NameSet (s x) dependent_vars) interesting_vars.
@@ -22,26 +27,34 @@ Definition substitute_term (s : substitution Name) (t : quantified_term) : quant
 Definition substitute_pattern (s : substitution Name) (p : quantified_pattern) : quantified_pattern :=
   fun v => p (fun x => s x v).
 
-Lemma substitute_term_dependent_vars s (t : quantified_term) t_vars s_vars :
+Lemma substitute_term_dependent_vars s (t : quantified_term) t_vars t_vars' s_vars s_vars' :
   pattern_dependent_vars NameSet t t_vars ->
-  substitution_dependent_vars s t_vars s_vars ->
-  pattern_dependent_vars NameSet (substitute_term s t) s_vars.
+  t_vars ⊆ t_vars' ->
+  substitution_dependent_vars s t_vars' s_vars ->
+  s_vars ⊆ s_vars' ->
+  pattern_dependent_vars NameSet (substitute_term s t) s_vars'.
 Proof.
-  intros Ht_deps Hs_deps v1 v2 Heqvars.
+  intros Ht_deps Ht Hs_deps Hs v1 v2 Heqvars.
   apply Ht_deps.
   constructor; intros x Hx.
-  by apply (Hs_deps x Hx _ _ Heqvars).
+  apply Ht in Hx.
+  eapply ARLVarsEqProper_subseteq in Heqvars; [| done..].
+  by eapply (Hs_deps x Hx _ _ Heqvars).
 Qed.
 
-Lemma substitute_pattern_dependent_vars s (t : quantified_pattern) t_vars s_vars :
+Lemma substitute_pattern_dependent_vars s (t : quantified_pattern) t_vars t_vars' s_vars s_vars' :
   pattern_dependent_vars NameSet t t_vars ->
-  substitution_dependent_vars s t_vars s_vars ->
-  pattern_dependent_vars NameSet (substitute_pattern s t) s_vars.
+  t_vars ⊆ t_vars' ->
+  substitution_dependent_vars s t_vars' s_vars ->
+  s_vars ⊆ s_vars' ->
+  pattern_dependent_vars NameSet (substitute_pattern s t) s_vars'.
 Proof.
-  intros Ht_deps Hs_deps v1 v2 Heqvars.
+  intros Ht_deps Ht Hs_deps Hs v1 v2 Heqvars.
   apply Ht_deps.
   constructor; intros x Hx.
-  by apply (Hs_deps x Hx _ _ Heqvars).
+  apply Ht in Hx.
+  eapply ARLVarsEqProper_subseteq in Heqvars; [| done..].
+  by eapply (Hs_deps x Hx _ _ Heqvars).
 Qed.
 
 Record Substitution :=
@@ -58,7 +71,7 @@ Lemma Substitute_term_dependent_vars s (t : quantified_term):
   pattern_dependent_vars NameSet (substitute_term s t) (sub_to s).
 Proof.
   intros.
-  by eapply substitute_term_dependent_vars, s.
+  by eapply substitute_term_dependent_vars; [..| apply s |].
 Qed.
 
 Lemma Substitute_pattern_dependent_vars s (t : quantified_pattern):
@@ -66,6 +79,16 @@ Lemma Substitute_pattern_dependent_vars s (t : quantified_pattern):
   pattern_dependent_vars NameSet (substitute_pattern s t) (sub_to s).
 Proof.
   intros.
-  by eapply substitute_pattern_dependent_vars, s.
+  by eapply substitute_pattern_dependent_vars; [..| apply s |].
 Qed.
 
+Record TermMatching
+  (patt : quantified_term) (patt_vars : NameSet) (s : Substitution)
+  (term : quantified_term): Prop :=
+{
+  tm_patt_dep_vars : pattern_dependent_vars NameSet patt patt_vars;
+  tm_subst_vars : sub_from s ⊆ patt_vars;
+  tm_patt_match : substitute_term s patt = term;
+}.
+
+End sec_matching.
